CertiGC/verif_resume.v
@@ -1,5 +1,24 @@
 Require Import RamifyCoq.CertiGC.gc_spec.
 
+Lemma generation_rep_memory_block: forall sh (g: LGraph) gen num,
+    (gen < length g.(glabel))%nat ->
+    generation_rep sh g (gen, num) |--
+    memory_block sh (previous_vertices_size g gen num) (gen_start g gen).
+Proof.
+  intros. assert (isptr (gen_start g gen)) by (apply start_isptr).
+  remember (gen_start g gen). destruct v; try (simpl in H0; exfalso; assumption).
+  induction num.
+  - simpl. rewrite memory_block_zero_Vptr. auto.
+  - unfold generation_rep. rewrite nat_inc_list_S, map_app, iter_sepcon_app_sepcon.
+    simpl. unfold generation_rep in IHnum. sep_apply IHnum. rewrite Z.add_comm.
+    rewrite <- (Ptrofs.repr_unsigned i) at 2. rewrite memory_block_split.
+    rewrite Ptrofs.repr_unsigned. entailer!. unfold vertex_rep, vertex_at. simpl.
+    unfold vertex_address. simpl vgeneration. rewrite <- Heqv. unfold vertex_offset.
+    simpl vgeneration. simpl vindex. rewrite offset_offset_val.
+    remember (previous_vertices_size g gen (vindex (gen, num))).
+    replace (WORD_SIZE * (z + 1) + - WORD_SIZE) with (WORD_SIZE * z)%Z.
+Abort.
+
 Lemma body_resume: semax_body Vprog Gprog f_resume resume_spec.
 Proof.
   start_function.
@@ -9,12 +28,27 @@ Proof.
   replace_SEP 1 (fun_info_rep rsh f_info fi) by unfold fun_info_rep; entailer!.
   forward_if True; [forward; entailer!|exfalso; destruct t_info; simpl in *; tauto|].
   Intros. remember (ti_heap_p t_info) as h. remember (ti_heap t_info) as th.
-  forward; rewrite Znth_0_cons.
-  - (* goal: is_pointer_or_null (space_start (heap_head (ti_heap t_info))) *)
-
+  assert_PROP (isptr (space_start (heap_head th))). {
     destruct H as [? [? ?]]. rewrite <- Heqh in *. rewrite <- Heqth in *.
-    remember (glabel g) as ginfo. destruct ginfo.
-    1: exfalso; apply H1; rewrite <- H; reflexivity. simpl in H2.
-    admit.
-  - 
+    unfold graph_rep. remember (glabel g) as ginfo. destruct ginfo.
+    1: exfalso; apply H1; rewrite <- H; reflexivity. simpl in * |-.
+    pose proof (spaces_size th). remember (spaces th). destruct l. 1: inversion H4.
+    rewrite map_cons in H3. rewrite Forall_forall in H2. simpl in H2.
+    assert (generation_space_compatible g (O, g0, s)) by (apply H2; left; reflexivity).
+    destruct H5 as [? [? ?]]. pose proof (start_isptr g0). rewrite H5 in H8.
+    entailer!. assert (heap_head (ti_heap t_info) = s). {
+      destruct (ti_heap t_info) eqn:? . simpl in Heql. unfold heap_head. simpl.
+      destruct spaces; inversion Heql. reflexivity.
+    } rewrite H17. assumption.
+  } forward. rewrite Znth_0_cons. forward. rewrite Znth_0_cons. forward_if True.
+  - remember (space_start (heap_head (ti_heap t_info))).
+    destruct v0; try (simpl in Heqv0; exfalso; assumption). unfold denote_tc_samebase.
+    simpl. entailer!.
+  - unfold all_string_constants. Intros.
+    forward_call ((gv ___stringlit_10),
+                  (map init_data2byte (gvar_init v___stringlit_10)), rsh).
+    exfalso; assumption.
+  - forward. entailer!.
+  - forward. forward.
+    
 Abort.
